solver is 3 and logic is DLA

SlowTest/DiffLogic-Test/seq_Boogie.bpl
@@ -1,29 +1,50 @@
-// procedure S1(len: int) returns (a: [int]bool);
-//   requires 0 < len;
-//   ensures (forall j: int :: 0 <= j && j < len ==> a[j]);
+type Val;
+procedure S0() returns (a: [Val]bool) // works
+{
+    var X: Val;
+    a[X] := true;
+    // assume a[X];
+    assert (forall j: Val :: j == X ==> a[j]);
+}
 
-// implementation S1(len: int) returns (a: [int]bool)
-// {
-//     var i: int;
-//     i := 0;
-//     a[0] := true;
-//     while ( i < len )
-//         invariant 0 <= i && i <= len;
-//         invariant (forall j: int :: 0 <= j && j < i ==> a[j]);
-//     {
-//         a[i] := true;
-//         assume (forall j: int :: i == j ==> a[j]);
-//         i := i + 1;
-//     }
-// }
+procedure S0'() returns (a: [int]bool)
+{
+    a[0] := true;
+    // assume a[X];
+    assert (forall j:int :: j == 0 ==> a[j]); // quantifier tactic?
+}
 
-procedure S2(in: [int]int, len: int) returns (out: [int]int);
-  requires in[0] == 0 && (forall i: int :: 0 <= i && i < len - 1 ==> in[i + 1] == in[i] + 1); // this `requires` works
-//   requires in[0] == 0 && (forall i: int :: 0 <= i ==> in[i + 1] == in[i] + 1); // this `requires` makes verification run forever
+procedure S1(len: int) returns (a: [int]bool)
+  requires 0 < len;
+  ensures (forall j: int :: 0 <= j && j < len ==> a[j]);
+{
+    var i: int;
+    i := 0;
+    a[0] := true;
+    while ( i < len )
+        invariant 0 <= i && i <= len;
+        invariant (forall j: int :: {a[j]} 0 <= j && j < i ==> a[j]);
+    {
+        a[i] := true;
+        // assume a[i]; // not work
+        // assert (forall j: int :: 0 <= j && j < i ==> a[j]);
+        // assume (forall j: int :: {a[j]} i == j ==> a[j]);
+
+        // assert (forall j: int :: i == j ==> 0 <= j && j < i + 1 ==> a[j]);
+        // assert (forall j: int :: i != j ==> 0 <= j && j < i + 1 ==> a[j]);
+
+        // assert (0 <= i && i < i + 1 ==> a[i]);
+
+        i := i + 1;
+    }
+}
+
+procedure S2(in: [int]int, len: int) returns (out: [int]int)
+//   requires in[0] == 0 && (forall i: int :: 0 <= i && i < len - 1 ==> in[i + 1] == in[i] + 1); // works
+//   requires in[0] == 0 && (forall i: int :: 0 <= i ==> in[i] == 1); // works
+  requires in[0] == 0 && (forall i: int :: {in[i] + 1} 0 <= i ==> in[i + 1] == in[i] + 1); // need trigger to work
   requires 0 < len;
   ensures (forall j: int :: 0 <= j && j < len ==> out[j] == in[j]);
-
-implementation S2(in: [int]int, len: int) returns (out: [int]int)
 {
     var i : int;
 
@@ -34,7 +55,7 @@ implementation S2(in: [int]int, len: int) returns (out: [int]int)
       invariant out[0] == 0 && (forall j: int :: 0 <= j && j < i ==> out[j] == in[j]);
     {
         out[i] := in[i];
-        assume (forall j: int :: i == j ==> out[j] == in[j]);
+        // assume (forall j: int :: i == j ==> out[j] == in[j]);
         i := i + 1;
     }
 
