SlowTest/DiffLogic-Test/seq-Boogie2z3.smt2
@@ -1,5 +1,6 @@
 (set-option :print-success false)
 (set-info :smt-lib-version 2.0)
+(set-option :smt.arith.solver 3)
 (set-option :AUTO_CONFIG false)
 (set-option :pp.bv_literals false)
 (set-option :MODEL.V2 true)
@@ -15,11 +16,198 @@
 (set-option :TYPE_CHECK true)
 (set-option :smt.BV.REFLECT true)
 (set-option :model.compact false)
+(set-logic DLA)
 ; done setting options
 
 
 (declare-fun tickleBool (Bool) Bool)
 (assert (and (tickleBool true) (tickleBool false)))
+(declare-fun %lbl%+0 () Bool)
+(declare-sort T@Val 0)
+(declare-sort |T@[Val]Bool| 0)
+(declare-fun a@0 () |T@[Val]Bool|)
+(declare-fun |Store_[Val]$bool| (|T@[Val]Bool| T@Val Bool) |T@[Val]Bool|)
+(declare-fun |Select_[Val]$bool| (|T@[Val]Bool| T@Val) Bool)
+(assert (forall ( ( ?x0 |T@[Val]Bool|) ( ?x1 T@Val) ( ?x2 Bool)) (= (|Select_[Val]$bool| (|Store_[Val]$bool| ?x0 ?x1 ?x2) ?x1)  ?x2)))
+(assert (forall ( ( ?x0 |T@[Val]Bool|) ( ?x1 T@Val) ( ?y1 T@Val) ( ?x2 Bool)) (=>  (not (= ?x1 ?y1)) (= (|Select_[Val]$bool| (|Store_[Val]$bool| ?x0 ?x1 ?x2) ?y1) (|Select_[Val]$bool| ?x0 ?y1)))))
+(declare-fun a () |T@[Val]Bool|)
+(declare-fun X () T@Val)
+(declare-fun %lbl%@1 () Bool)
+(declare-fun %lbl%+2 () Bool)
+(push 1)
+(set-info :boogie-vc-id S0)
+(assert (not
+(let ((anon0_correct  (=> (! (and %lbl%+0 true) :lblpos +0) (=> (= a@0 (|Store_[Val]$bool| a X true)) (! (or %lbl%@1 (forall ((j T@Val) ) (!  (=> (= j X) (|Select_[Val]$bool| a@0 j))
+ :qid |seqBoogi.7:20|
+ :skolemid |0|
+))) :lblneg @1)))))
+(let ((PreconditionGeneratedEntry_correct  (=> (! (and %lbl%+2 true) :lblpos +2) anon0_correct)))
+PreconditionGeneratedEntry_correct))
+))
+(check-sat)
+(pop 1)
+; Valid
+(reset)
+(set-option :print-success false)
+(set-info :smt-lib-version 2.0)
+(set-option :smt.arith.solver 3)
+(set-option :AUTO_CONFIG false)
+(set-option :pp.bv_literals false)
+(set-option :MODEL.V2 true)
+(set-option :smt.PHASE_SELECTION 0)
+(set-option :smt.RESTART_STRATEGY 0)
+(set-option :smt.RESTART_FACTOR |1.5|)
+(set-option :smt.ARITH.RANDOM_INITIAL_VALUE true)
+(set-option :smt.CASE_SPLIT 3)
+(set-option :smt.DELAY_UNITS true)
+(set-option :NNF.SK_HACK true)
+(set-option :smt.MBQI false)
+(set-option :smt.QI.EAGER_THRESHOLD 100)
+(set-option :TYPE_CHECK true)
+(set-option :smt.BV.REFLECT true)
+(set-option :model.compact false)
+(set-logic DLA)
+; done setting options
+
+
+(declare-fun tickleBool (Bool) Bool)
+(assert (and (tickleBool true) (tickleBool false)))
+; Valid
+
+(declare-fun %lbl%+0 () Bool)
+(declare-sort |T@[Int]Bool| 0)
+(declare-fun a@0 () |T@[Int]Bool|)
+(declare-fun |Store_[$int]$bool| (|T@[Int]Bool| Int Bool) |T@[Int]Bool|)
+(declare-fun |Select_[$int]$bool| (|T@[Int]Bool| Int) Bool)
+(assert (forall ( ( ?x0 |T@[Int]Bool|) ( ?x1 Int) ( ?x2 Bool)) (= (|Select_[$int]$bool| (|Store_[$int]$bool| ?x0 ?x1 ?x2) ?x1)  ?x2)))
+(assert (forall ( ( ?x0 |T@[Int]Bool|) ( ?x1 Int) ( ?y1 Int) ( ?x2 Bool)) (=>  (not (= ?x1 ?y1)) (= (|Select_[$int]$bool| (|Store_[$int]$bool| ?x0 ?x1 ?x2) ?y1) (|Select_[$int]$bool| ?x0 ?y1)))))
+(declare-fun a () |T@[Int]Bool|)
+(declare-fun %lbl%@1 () Bool)
+(declare-fun %lbl%+2 () Bool)
+(push 1)
+(set-info :boogie-vc-id |S0'|)
+(assert (not
+(let ((anon0_correct  (=> (! (and %lbl%+0 true) :lblpos +0) (=> (= a@0 (|Store_[$int]$bool| a 0 true)) (! (or %lbl%@1 (forall ((j Int) ) (!  (=> (= j 0) (|Select_[$int]$bool| a@0 j))
+ :qid |seqBoogi.14:20|
+ :skolemid |1|
+))) :lblneg @1)))))
+(let ((PreconditionGeneratedEntry_correct  (=> (! (and %lbl%+2 true) :lblpos +2) anon0_correct)))
+PreconditionGeneratedEntry_correct))
+))
+(check-sat)
+(pop 1)
+; Valid
+(reset)
+(set-option :print-success false)
+(set-info :smt-lib-version 2.0)
+(set-option :smt.arith.solver 3)
+(set-option :AUTO_CONFIG false)
+(set-option :pp.bv_literals false)
+(set-option :MODEL.V2 true)
+(set-option :smt.PHASE_SELECTION 0)
+(set-option :smt.RESTART_STRATEGY 0)
+(set-option :smt.RESTART_FACTOR |1.5|)
+(set-option :smt.ARITH.RANDOM_INITIAL_VALUE true)
+(set-option :smt.CASE_SPLIT 3)
+(set-option :smt.DELAY_UNITS true)
+(set-option :NNF.SK_HACK true)
+(set-option :smt.MBQI false)
+(set-option :smt.QI.EAGER_THRESHOLD 100)
+(set-option :TYPE_CHECK true)
+(set-option :smt.BV.REFLECT true)
+(set-option :model.compact false)
+(set-logic DLA)
+; done setting options
+
+
+(declare-fun tickleBool (Bool) Bool)
+(assert (and (tickleBool true) (tickleBool false)))
+; Valid
+
+(declare-fun %lbl%+0 () Bool)
+(declare-fun %lbl%@1 () Bool)
+(declare-fun len () Int)
+(declare-sort |T@[Int]Bool| 0)
+(declare-fun |Select_[$int]$bool| (|T@[Int]Bool| Int) Bool)
+(declare-fun a@3 () |T@[Int]Bool|)
+(declare-fun %lbl%+2 () Bool)
+(declare-fun i@0 () Int)
+(declare-fun a@1 () |T@[Int]Bool|)
+(declare-fun %lbl%+3 () Bool)
+(declare-fun a@2 () |T@[Int]Bool|)
+(declare-fun |Store_[$int]$bool| (|T@[Int]Bool| Int Bool) |T@[Int]Bool|)
+(assert (forall ( ( ?x0 |T@[Int]Bool|) ( ?x1 Int) ( ?x2 Bool)) (= (|Select_[$int]$bool| (|Store_[$int]$bool| ?x0 ?x1 ?x2) ?x1)  ?x2)))
+(assert (forall ( ( ?x0 |T@[Int]Bool|) ( ?x1 Int) ( ?y1 Int) ( ?x2 Bool)) (=>  (not (= ?x1 ?y1)) (= (|Select_[$int]$bool| (|Store_[$int]$bool| ?x0 ?x1 ?x2) ?y1) (|Select_[$int]$bool| ?x0 ?y1)))))
+(declare-fun i@1 () Int)
+(declare-fun %lbl%@4 () Bool)
+(declare-fun %lbl%@5 () Bool)
+(declare-fun %lbl%+6 () Bool)
+(declare-fun %lbl%+7 () Bool)
+(declare-fun a@0 () |T@[Int]Bool|)
+(declare-fun a () |T@[Int]Bool|)
+(declare-fun %lbl%@8 () Bool)
+(declare-fun %lbl%@9 () Bool)
+(declare-fun %lbl%+10 () Bool)
+(push 1)
+(set-info :boogie-vc-id S1)
+(assert (not
+(let ((GeneratedUnifiedExit_correct  (=> (! (and %lbl%+0 true) :lblpos +0) (! (or %lbl%@1 (forall ((j Int) ) (!  (=> (and (<= 0 j) (< j len)) (|Select_[$int]$bool| a@3 j))
+ :qid |seqBoogi.19:19|
+ :skolemid |2|
+))) :lblneg @1))))
+(let ((anon2_LoopDone_correct  (=> (! (and %lbl%+2 true) :lblpos +2) (=> (and (<= len i@0) (= a@3 a@1)) GeneratedUnifiedExit_correct))))
+(let ((anon2_LoopBody_correct  (=> (! (and %lbl%+3 true) :lblpos +3) (=> (< i@0 len) (=> (and (= a@2 (|Store_[$int]$bool| a@1 i@0 true)) (= i@1 (+ i@0 1))) (and (! (or %lbl%@4  (and (<= 0 i@1) (<= i@1 len))) :lblneg @4) (=> (and (<= 0 i@1) (<= i@1 len)) (! (or %lbl%@5 (forall ((j@@0 Int) ) (!  (=> (and (<= 0 j@@0) (< j@@0 i@1)) (|Select_[$int]$bool| a@2 j@@0))
+ :qid |seqBoogi.26:27|
+ :skolemid |3|
+ :pattern ( (|Select_[$int]$bool| a@2 j@@0))
+))) :lblneg @5))))))))
+(let ((anon2_LoopHead_correct  (=> (! (and %lbl%+6 true) :lblpos +6) (=> (<= 0 i@0) (=> (and (and (<= 0 i@0) (<= i@0 len)) (forall ((j@@1 Int) ) (!  (=> (and (<= 0 j@@1) (< j@@1 i@0)) (|Select_[$int]$bool| a@1 j@@1))
+ :qid |seqBoogi.26:27|
+ :skolemid |3|
+ :pattern ( (|Select_[$int]$bool| a@1 j@@1))
+))) (and anon2_LoopDone_correct anon2_LoopBody_correct))))))
+(let ((anon0_correct  (=> (! (and %lbl%+7 true) :lblpos +7) (=> (= a@0 (|Store_[$int]$bool| a 0 true)) (and (! (or %lbl%@8  (and (<= 0 0) (<= 0 len))) :lblneg @8) (=> (and (<= 0 0) (<= 0 len)) (and (! (or %lbl%@9 (forall ((j@@2 Int) ) (!  (=> (and (<= 0 j@@2) (< j@@2 0)) (|Select_[$int]$bool| a@0 j@@2))
+ :qid |seqBoogi.26:27|
+ :skolemid |3|
+ :pattern ( (|Select_[$int]$bool| a@0 j@@2))
+))) :lblneg @9) (=> (forall ((j@@3 Int) ) (!  (=> (and (<= 0 j@@3) (< j@@3 0)) (|Select_[$int]$bool| a@0 j@@3))
+ :qid |seqBoogi.26:27|
+ :skolemid |3|
+ :pattern ( (|Select_[$int]$bool| a@0 j@@3))
+)) anon2_LoopHead_correct))))))))
+(let ((PreconditionGeneratedEntry_correct  (=> (! (and %lbl%+10 true) :lblpos +10) (=> (< 0 len) anon0_correct))))
+PreconditionGeneratedEntry_correct))))))
+))
+(check-sat)
+(pop 1)
+; Valid
+(reset)
+(set-option :print-success false)
+(set-info :smt-lib-version 2.0)
+(set-option :smt.arith.solver 3)
+(set-option :AUTO_CONFIG false)
+(set-option :pp.bv_literals false)
+(set-option :MODEL.V2 true)
+(set-option :smt.PHASE_SELECTION 0)
+(set-option :smt.RESTART_STRATEGY 0)
+(set-option :smt.RESTART_FACTOR |1.5|)
+(set-option :smt.ARITH.RANDOM_INITIAL_VALUE true)
+(set-option :smt.CASE_SPLIT 3)
+(set-option :smt.DELAY_UNITS true)
+(set-option :NNF.SK_HACK true)
+(set-option :smt.MBQI false)
+(set-option :smt.QI.EAGER_THRESHOLD 100)
+(set-option :TYPE_CHECK true)
+(set-option :smt.BV.REFLECT true)
+(set-option :model.compact false)
+(set-logic DLA)
+; done setting options
+
+
+(declare-fun tickleBool (Bool) Bool)
+(assert (and (tickleBool true) (tickleBool false)))
+; Valid
+
 (declare-fun %lbl%+0 () Bool)
 (declare-fun %lbl%@1 () Bool)
 (declare-fun len () Int)
@@ -58,46 +246,44 @@
 (set-info :boogie-vc-id S2)
 (assert (not
 (let ((GeneratedUnifiedExit_correct  (=> (! (and %lbl%+0 true) :lblpos +0) (! (or %lbl%@1 (forall ((j Int) ) (!  (=> (and (<= 0 j) (< j len)) (= (|Select_[$int]$int| out@3 j) (|Select_[$int]$int| in j)))
- :qid |seqBoogi.24:19|
- :skolemid |1|
+ :qid |seqBoogi.47:19|
+ :skolemid |5|
 ))) :lblneg @1))))
 (let ((anon5_LoopDone_correct  (=> (! (and %lbl%+2 true) :lblpos +2) (=> (and (<= len i@2) (= out@3 out@1)) GeneratedUnifiedExit_correct))))
 (let ((anon5_LoopBody_correct  (=> (! (and %lbl%+3 true) :lblpos +3) (=> (and (< i@2 len) (= i@3 (+ i@2 1))) (and (! (or %lbl%@4  (and (<= 0 i@3) (<= i@3 len))) :lblneg @4) (=> (and (<= 0 i@3) (<= i@3 len)) (! (or %lbl%@5 (forall ((j@@0 Int) ) (!  (=> (and (<= 0 j@@0) (< j@@0 i@3)) (= (|Select_[$int]$int| out@1 j@@0) (|Select_[$int]$int| in j@@0)))
- :qid |seqBoogi.44:25|
- :skolemid |4|
+ :qid |seqBoogi.65:25|
+ :skolemid |7|
 ))) :lblneg @5)))))))
 (let ((anon5_LoopHead_correct  (=> (! (and %lbl%+6 true) :lblpos +6) (=> (<= 0 i@2) (=> (and (and (<= 0 i@2) (<= i@2 len)) (forall ((j@@1 Int) ) (!  (=> (and (<= 0 j@@1) (< j@@1 i@2)) (= (|Select_[$int]$int| out@1 j@@1) (|Select_[$int]$int| in j@@1)))
- :qid |seqBoogi.44:25|
- :skolemid |4|
+ :qid |seqBoogi.65:25|
+ :skolemid |7|
 ))) (and anon5_LoopDone_correct anon5_LoopBody_correct))))))
 (let ((anon4_LoopDone_correct  (=> (! (and %lbl%+7 true) :lblpos +7) (=> (<= len i@0) (and (! (or %lbl%@8  (and (<= 0 0) (<= 0 len))) :lblneg @8) (=> (and (<= 0 0) (<= 0 len)) (and (! (or %lbl%@9 (forall ((j@@2 Int) ) (!  (=> (and (<= 0 j@@2) (< j@@2 0)) (= (|Select_[$int]$int| out@1 j@@2) (|Select_[$int]$int| in j@@2)))
- :qid |seqBoogi.44:25|
- :skolemid |4|
+ :qid |seqBoogi.65:25|
+ :skolemid |7|
 ))) :lblneg @9) (=> (forall ((j@@3 Int) ) (!  (=> (and (<= 0 j@@3) (< j@@3 0)) (= (|Select_[$int]$int| out@1 j@@3) (|Select_[$int]$int| in j@@3)))
- :qid |seqBoogi.44:25|
- :skolemid |4|
+ :qid |seqBoogi.65:25|
+ :skolemid |7|
 )) anon5_LoopHead_correct))))))))
-(let ((anon4_LoopBody_correct  (=> (! (and %lbl%+10 true) :lblpos +10) (=> (and (and (< i@0 len) (= out@2 (|Store_[$int]$int| out@1 i@0 (|Select_[$int]$int| in i@0)))) (and (forall ((j@@4 Int) ) (!  (=> (= i@0 j@@4) (= (|Select_[$int]$int| out@2 j@@4) (|Select_[$int]$int| in j@@4)))
- :qid |seqBoogi.37:24|
- :skolemid |3|
-)) (= i@1 (+ i@0 1)))) (and (! (or %lbl%@11  (and (<= 0 i@1) (<= i@1 len))) :lblneg @11) (=> (and (<= 0 i@1) (<= i@1 len)) (! (or %lbl%@12  (and (= (|Select_[$int]$int| out@2 0) 0) (forall ((j@@5 Int) ) (!  (=> (and (<= 0 j@@5) (< j@@5 i@1)) (= (|Select_[$int]$int| out@2 j@@5) (|Select_[$int]$int| in j@@5)))
- :qid |seqBoogi.34:40|
- :skolemid |2|
-)))) :lblneg @12)))))))
-(let ((anon4_LoopHead_correct  (=> (! (and %lbl%+13 true) :lblpos +13) (=> (<= 0 i@0) (=> (and (and (<= 0 i@0) (<= i@0 len)) (and (= (|Select_[$int]$int| out@1 0) 0) (forall ((j@@6 Int) ) (!  (=> (and (<= 0 j@@6) (< j@@6 i@0)) (= (|Select_[$int]$int| out@1 j@@6) (|Select_[$int]$int| in j@@6)))
- :qid |seqBoogi.34:40|
- :skolemid |2|
+(let ((anon4_LoopBody_correct  (=> (! (and %lbl%+10 true) :lblpos +10) (=> (< i@0 len) (=> (and (= out@2 (|Store_[$int]$int| out@1 i@0 (|Select_[$int]$int| in i@0))) (= i@1 (+ i@0 1))) (and (! (or %lbl%@11  (and (<= 0 i@1) (<= i@1 len))) :lblneg @11) (=> (and (<= 0 i@1) (<= i@1 len)) (! (or %lbl%@12  (and (= (|Select_[$int]$int| out@2 0) 0) (forall ((j@@4 Int) ) (!  (=> (and (<= 0 j@@4) (< j@@4 i@1)) (= (|Select_[$int]$int| out@2 j@@4) (|Select_[$int]$int| in j@@4)))
+ :qid |seqBoogi.55:40|
+ :skolemid |6|
+)))) :lblneg @12))))))))
+(let ((anon4_LoopHead_correct  (=> (! (and %lbl%+13 true) :lblpos +13) (=> (<= 0 i@0) (=> (and (and (<= 0 i@0) (<= i@0 len)) (and (= (|Select_[$int]$int| out@1 0) 0) (forall ((j@@5 Int) ) (!  (=> (and (<= 0 j@@5) (< j@@5 i@0)) (= (|Select_[$int]$int| out@1 j@@5) (|Select_[$int]$int| in j@@5)))
+ :qid |seqBoogi.55:40|
+ :skolemid |6|
 )))) (and anon4_LoopDone_correct anon4_LoopBody_correct))))))
-(let ((anon0_correct  (=> (! (and %lbl%+14 true) :lblpos +14) (=> (= out@0 (|Store_[$int]$int| out 0 0)) (and (! (or %lbl%@15  (and (<= 0 0) (<= 0 len))) :lblneg @15) (=> (and (<= 0 0) (<= 0 len)) (and (! (or %lbl%@16  (and (= (|Select_[$int]$int| out@0 0) 0) (forall ((j@@7 Int) ) (!  (=> (and (<= 0 j@@7) (< j@@7 0)) (= (|Select_[$int]$int| out@0 j@@7) (|Select_[$int]$int| in j@@7)))
- :qid |seqBoogi.34:40|
- :skolemid |2|
-)))) :lblneg @16) (=> (and (= (|Select_[$int]$int| out@0 0) 0) (forall ((j@@8 Int) ) (!  (=> (and (<= 0 j@@8) (< j@@8 0)) (= (|Select_[$int]$int| out@0 j@@8) (|Select_[$int]$int| in j@@8)))
- :qid |seqBoogi.34:40|
- :skolemid |2|
+(let ((anon0_correct  (=> (! (and %lbl%+14 true) :lblpos +14) (=> (= out@0 (|Store_[$int]$int| out 0 0)) (and (! (or %lbl%@15  (and (<= 0 0) (<= 0 len))) :lblneg @15) (=> (and (<= 0 0) (<= 0 len)) (and (! (or %lbl%@16  (and (= (|Select_[$int]$int| out@0 0) 0) (forall ((j@@6 Int) ) (!  (=> (and (<= 0 j@@6) (< j@@6 0)) (= (|Select_[$int]$int| out@0 j@@6) (|Select_[$int]$int| in j@@6)))
+ :qid |seqBoogi.55:40|
+ :skolemid |6|
+)))) :lblneg @16) (=> (and (= (|Select_[$int]$int| out@0 0) 0) (forall ((j@@7 Int) ) (!  (=> (and (<= 0 j@@7) (< j@@7 0)) (= (|Select_[$int]$int| out@0 j@@7) (|Select_[$int]$int| in j@@7)))
+ :qid |seqBoogi.55:40|
+ :skolemid |6|
 ))) anon4_LoopHead_correct))))))))
-(let ((PreconditionGeneratedEntry_correct  (=> (! (and %lbl%+17 true) :lblpos +17) (=> (and (and (= (|Select_[$int]$int| in 0) 0) (forall ((i Int) ) (!  (=> (and (<= 0 i) (< i (- len 1))) (= (|Select_[$int]$int| in (+ i 1)) (+ (|Select_[$int]$int| in i) 1)))
- :qid |seqBoogi.21:34|
- :skolemid |0|
+(let ((PreconditionGeneratedEntry_correct  (=> (! (and %lbl%+17 true) :lblpos +17) (=> (and (and (= (|Select_[$int]$int| in 0) 0) (forall ((i Int) ) (!  (=> (<= 0 i) (= (|Select_[$int]$int| in (+ i 1)) (+ (|Select_[$int]$int| in i) 1)))
+ :qid |seqBoogi.45:34|
+ :skolemid |4|
+ :pattern ( (+ (|Select_[$int]$int| in i) 1))
 ))) (< 0 len)) anon0_correct))))
 PreconditionGeneratedEntry_correct)))))))))
 ))
